Split up recovery and crash dependencies.

src/program_logic/staged_invariant.v
@@ -4,38 +4,9 @@ From stdpp Require Export namespaces.
 From iris.base_logic.lib Require Import wsat invariants saved_prop.
 From iris.algebra Require Import gmap.
 From iris.proofmode Require Import tactics.
-From Perennial.program_logic Require Export step_fupd_extra.
+From Perennial.program_logic Require Export step_fupd_extra crash_token.
 Set Default Proof Using "Type".
 Import uPred.
-
-Definition crashR := csumR (exclR unitO) (agreeR unitO).
-Definition NC_tok : crashR := Cinl (Excl ()).
-Definition C_tok : crashR := Cinr (to_agree ()).
-
-Class crashG Σ := { crash_inG :> inG Σ crashR; crash_name : gname }.
-Class crashPreG Σ := { crash_inPreG :> inG Σ crashR }.
-
-Definition crashΣ : gFunctors :=
-    #[GFunctor (csumR (exclR unitO) (agreeR unitO))].
-
-Instance subG_crashG {Σ} : subG crashΣ Σ → crashPreG Σ.
-Proof. solve_inG. Qed.
-
-Definition NC_def `{crashG Σ} := own crash_name NC_tok.
-Definition NC_aux `{crashG Σ} : seal NC_def. by eexists. Qed.
-Definition NC `{crashG Σ} := NC_aux.(unseal).
-Definition C_def `{crashG Σ} := own crash_name C_tok.
-Definition C_aux `{crashG Σ} : seal C_def. by eexists. Qed.
-Definition C `{crashG Σ} := C_aux.(unseal).
-
-Lemma NC_alloc `{!crashPreG Σ} : (|==> ∃ _ : crashG Σ, NC)%I.
-Proof.
-  iIntros.
-  iMod (own_alloc (Cinl (Excl ()))) as (γ) "H".
-  { econstructor. }
-  iExists {| crash_name := γ |}.
-  rewrite /NC NC_aux.(seal_eq). by iFrame.
-Qed.
 
 Class stagedG (Σ : gFunctors) : Set := WsatG {
   staging_saved_inG :> savedPropG Σ;
@@ -64,32 +35,6 @@ Context `{!invG Σ, !stagedG Σ, !crashG Σ}.
 Implicit Types i : positive.
 Implicit Types N : namespace.
 Implicit Types P Q R : iProp Σ.
-
-Global Instance C_timeless : Timeless C.
-Proof. rewrite /C C_aux.(seal_eq). apply _. Qed.
-
-Global Instance C_persistent : Persistent C.
-Proof. rewrite /C C_aux.(seal_eq). apply _. Qed.
-
-Global Instance NC_timeless : Timeless NC.
-Proof. rewrite /NC NC_aux.(seal_eq). apply _. Qed.
-
-Lemma NC_C: NC -∗ C -∗ False.
-Proof.
- rewrite /C C_aux.(seal_eq).
- rewrite /NC NC_aux.(seal_eq).
-  iIntros "H H'".
-  { by iDestruct (own_valid_2 with "H H'") as %?. }
-Qed.
-
-Lemma NC_upd_C: NC ==∗ C.
-Proof.
- rewrite /C C_aux.(seal_eq).
- rewrite /NC NC_aux.(seal_eq).
- iIntros "H". iMod (own_update with "H") as "$".
- { by apply cmra_update_exclusive. }
- done.
-Qed.
 
 Global Instance staged_contractive N k E E' γ γ' : Contractive (staged_inv N k E E' γ γ').
 Proof.
@@ -131,7 +76,7 @@ Lemma staged_inv_iff N k E E' γ γ' P Q :
 Proof.
   iIntros "#HPQ". iApply inv_iff. iNext. iAlways. iSplit.
   - iIntros "H". iDestruct "H" as (?? P0 P0') "(?&?&?&#HP0&Hcase)". iExists _, _, P0, P0'. iFrame.
-    iAlways. iIntros. iSpecialize ("HP0" with "[$] [$]"). 
+    iAlways. iIntros. iSpecialize ("HP0" with "[$] [$]").
     iApply (step_fupdN_inner_wand' with "HP0"); eauto.
     iIntros "(?&$)". by iApply "HPQ".
   - iIntros "H". iDestruct "H" as (?? P0 P0') "(?&?&?&#HP0&Hcase)". iExists _, _, P0, P0'. iFrame.
@@ -240,37 +185,5 @@ Proof.
   { iNext. iExists _, _, _, _. iFrame "Hγ'". iFrame "#". by iRight. }
   iModIntro. eauto.
 Qed.
-
-(*
-Global Instance into_inv_staged_inv1 N γ P : IntoInv (staged_inv N γ P) N := {}.
-
-Definition staged_inv_exact N Pweak P :=
-  (∃ γ, staged_inv N γ Pweak ∗ staged_value N γ P)%I.
-*)
-
-(*
-Global Instance into_acc_inv E N γ Pweak P :
-  IntoAcc (staged_inv_exact N γ Pweak P)
-          (↑N ⊆ E) True (fupd E (E∖↑N)) (fupd (E∖↑N) E)
-          (λ _, ▷ ▷ P)%I (λ Q, Q ∗ ▷ P)%I (λ Q, Some (staged_value N γ Q))%I.
-Proof.
-  rewrite /IntoAcc /accessor.
-  iIntros (?) "(#Hinv&Hvalue) _". iMod (staged_inv_open with "[Hvalue]") as "($&?)"; first done.
-  { by iFrame. }
-  simpl default.
-  { auto.
-
-  i
-
-                                                                 Apply inv_open; done.
-Qed.
-
-Lemma inv_open_timeless E N P `{!Timeless P} :
-  ↑N ⊆ E → inv N P ={E,E∖↑N}=∗ P ∗ (P ={E∖↑N,E}=∗ True).
-Proof.
-  iIntros (?) "Hinv". iMod (inv_open with "Hinv") as "[>HP Hclose]"; auto.
-  iIntros "!> {$HP} HP". iApply "Hclose"; auto.
-Qed.
-*)
 
 End inv.
