src/program_logic/recovery_weakestpre.v
@@ -1,0 +1,99 @@
+From iris.proofmode Require Import tactics.
+From iris.algebra Require Import gmap auth agree gset coPset.
+From iris.base_logic.lib Require Import wsat.
+From iris.program_logic Require Export weakestpre.
+From Perennial.program_logic Require Export staged_invariant crash_lang crash_weakestpre.
+Import uPred.
+(*** Recovery ***)
+
+Class pbundleG (T: ofeT) (Σ: gFunctors) := {
+  pbundleT : T
+}.
+
+Class perennialG (Λ : language) (CS: crash_semantics Λ) (T: ofeT) (Σ : gFunctors) := PerennialG {
+  perennial_irisG :> ∀ (H: invG Σ), pbundleG T Σ → irisG Λ Σ;
+  perennial_invG: ∀ H t, @iris_invG _ _ (perennial_irisG H t) = H
+}.
+
+Definition wpr_pre `{perennialG Λ CS T Σ} (s : stuckness) (k: nat)
+    (wpr : invG Σ -d> crashG Σ -d> pbundleG T Σ -d> coPset -d> expr Λ -d> expr Λ -d> (val Λ -d> iPropO Σ) -d>
+                     (invG Σ -d> pbundleG T Σ -d> val Λ -d> iPropO Σ) -d> iPropO Σ) :
+  invG Σ -d> crashG Σ -d> pbundleG T Σ -d> coPset -d> expr Λ -d> expr Λ -d> (val Λ -d> iPropO Σ) -d> (invG Σ -d> pbundleG T Σ -d> val Λ -d> iPropO Σ) -d> iPropO Σ :=
+  λ H1 H2 t E e rec Φ Φr,
+  (WPC e @ s ; k; E ; ∅
+     {{ Φ }}
+     {{ ∀ σ σ' (HC: crash_prim_step CS σ σ') κs n,
+        state_interp σ κs n ={∅}=∗  ▷ ∀ H1 H2, NC -∗ ∃ t, state_interp σ' κs 0 ∗ wpr H1 H2 t E rec rec (λ v, Φr H1 t v) Φr ∗ NC}})%I.
+
+Local Instance wpr_pre_contractive `{!perennialG Λ CS T Σ} s k: Contractive (wpr_pre s k).
+Proof.
+  rewrite /wpr_pre=> n wp wp' Hwp ?? t E1 e1 rec Φ Φc.
+  apply wpc_ne; eauto;
+  repeat (f_contractive || f_equiv). apply Hwp.
+Qed.
+
+Definition wpr_def `{!perennialG Λ CS T Σ} (s : stuckness) k :
+  invG Σ → crashG Σ → pbundleG T Σ → coPset → expr Λ → expr Λ → (val Λ → iProp Σ) → (invG Σ → pbundleG T Σ → val Λ → iProp Σ) → iProp Σ := fixpoint (wpr_pre s k).
+Definition wpr_aux `{!perennialG Λ CS T Σ} : seal (@wpr_def Λ CS T Σ _). by eexists. Qed.
+Definition wpr `{!perennialG Λ CS T Σ} := wpr_aux.(unseal).
+Definition wpr_eq `{!perennialG Λ CS T Σ} : wpr = @wpr_def Λ CS T Σ _ := wpr_aux.(seal_eq).
+
+Section wpr.
+Context `{!perennialG Λ CS T Σ}.
+Implicit Types s : stuckness.
+Implicit Types k : nat.
+Implicit Types P : iProp Σ.
+Implicit Types Φ : val Λ → iProp Σ.
+Implicit Types Φc : invG Σ → pbundleG T Σ → val Λ → iProp Σ.
+Implicit Types v : val Λ.
+Implicit Types e : expr Λ.
+
+Lemma wpr_unfold s k Hi Hc t E e rec Φ Φc :
+  wpr s k Hi Hc t E e rec Φ Φc ⊣⊢ wpr_pre s k (wpr s k) Hi Hc t E e rec Φ Φc.
+Proof. rewrite wpr_eq. apply (fixpoint_unfold (wpr_pre s k)). Qed.
+
+(* There's a stronger version of this *)
+Lemma wpr_strong_mono s k Hi Hc t E e rec Φ Ψ Φr Ψr :
+  wpr s k Hi Hc t E e rec Φ Φr -∗
+  (∀ v, Φ v ==∗ Ψ v) ∧ (∀ Hi t v, Φr Hi t v ==∗ Ψr Hi t v) -∗
+  wpr s k Hi Hc t E e rec Ψ Ψr.
+Proof.
+  iIntros "H HΦ". iLöb as "IH" forall (e t Hi Hc E Φ Ψ Φr Ψr).
+  rewrite ?wpr_unfold /wpr_pre.
+  iApply (wpc_strong_mono' with "H") ; auto.
+  iSplit.
+  { iDestruct "HΦ" as "(H&_)". iIntros. iMod ("H" with "[$]"); eauto. }
+  iIntros "H".
+  rewrite difference_diag_L.
+  iModIntro. iIntros (?????) "Hinterp". iMod ("H" with "[//] Hinterp") as "H".
+  iModIntro. iNext. iIntros (Hi' Hc') "HNC". iDestruct ("H" $! Hi' Hc' with "[$]") as (?) "(?&H&HNC)".
+  iExists _. iFrame. iApply ("IH" with "[$]").
+  iSplit; iIntros; iDestruct ("HΦ") as "(_&H)"; by iMod ("H" with "[$]").
+Qed.
+
+(* To prove a recovery wp for e with rec, it suffices to prove a crash wp for e,
+   where the crash condition implies the precondition for a crash wp for rec *)
+Lemma idempotence_wpr s k E e rec Φx Φrx Φcx Hi Hc t:
+  ((WPC e @ s ; k ; E ; ∅ {{ Φx t }} {{ Φcx t }}) -∗
+   (□ ∀ (H: invG Σ) (Hc: crashG Σ) (t: pbundleG T Σ) σ σ' (HC: crash_prim_step CS σ σ') κs n,
+        Φcx t -∗ state_interp σ κs n ={∅}=∗
+        ▷ ∀ H' (Hc': crashG Σ), NC -∗ ∃ t', state_interp σ' κs 0 ∗ WPC rec @ s ; k; E ; ∅ {{ Φrx H' t' }} {{ Φcx t' }} ∗ NC) -∗
+    wpr s k Hi Hc t E e rec (Φx t) Φrx)%I.
+Proof.
+  iLöb as "IH" forall (E e Hi Hc t Φx).
+  iIntros "He #Hidemp".
+  rewrite wpr_unfold. rewrite /wpr_pre.
+  iApply (wpc_strong_mono' with "He"); [ auto | auto | auto | set_solver+ | ].
+  iSplit; first auto. iIntros "Hcx".
+  rewrite difference_diag_L.
+  iModIntro.
+  iIntros. iMod ("Hidemp" with "[ ] [$] [$]") as "H".
+  { eauto. }
+  iModIntro. iNext. iIntros (Hi' Hc') "HNC". iDestruct ("H" $! Hi' Hc' with "[$]") as (t') "(?&Hc&HNC)".
+  iExists _. iFrame.
+  iApply ("IH" $! E rec Hi' Hc' t' (λ t v, Φrx Hi' t v)%I with "[Hc]").
+  { iApply (wpc_strong_mono' with "Hc"); rewrite ?difference_diag_L; auto. }
+  eauto.
+Qed.
+
+End wpr.
